fix lawful circuit experiment

Clean/Examples/Add32LawfulCircuit.lean
@@ -8,27 +8,28 @@ open Gadgets.Addition32Full (add32_full Inputs)
 
 -- `infer_explicit_circuit` seem to work for all circuits
 instance explicit : ConstantExplicitCircuits (add32_full (p:=p)) := by
-  apply ConstantExplicitCircuits.from_constant_length (by infer_explicit_circuit)
-  try intros
-  simp only [ExplicitCircuit.local_length]
-  ac_rfl
+  infer_constant_explicit_circuits
 
 @[reducible] def circuit32 input := add32_full (p:=p) input
-#eval ExplicitCircuit.local_length (circuit32 default) 0
-#eval ExplicitCircuit.output (circuit32 default) 0
 
-example : ExplicitCircuit.final_offset (circuit32 default) 0 = 8 := by
-  dsimp only [explicit_norm, explicit, Boolean.circuit]
+example : ExplicitCircuit.local_length (circuit32 default) 0 = 8 := by
+  dsimp only [lawful_norm, explicit, Boolean.circuit]
 
 example : ExplicitCircuit.output (circuit32 default) 0
     = { z := { x0 := var ⟨0⟩, x1 := var ⟨2⟩, x2 := var ⟨4⟩, x3 := var ⟨6⟩ }, carry_out := var ⟨7⟩ } := by
-  dsimp only [explicit_norm, explicit, Boolean.circuit]
+  dsimp only [lawful_norm, explicit, Boolean.circuit]
 
-example (input : Var Inputs (F p)) (env) (i0 : ℕ) :
-    Circuit.constraints_hold.soundness env ((circuit32 input).operations i0) := by
-  let ⟨ x, y, carry_in ⟩ := input
-  let ⟨ x0, x1, x2, x3 ⟩ := x
-  let ⟨ y0, y1, y2, y3 ⟩ := y
+example (x0 x1 x2 x3 y0 y1 y2 y3 carry_in : Var field (F p)) env (i0 : ℕ) :
+  Circuit.constraints_hold.soundness env ((circuit32 ⟨ ⟨ x0, x1, x2, x3 ⟩, ⟨ y0, y1, y2, y3 ⟩, carry_in ⟩).operations i0)
+  ↔
+  (ZMod.val (env.get i0) < 256 ∧ (env.get (i0 + 1) = 0 ∨ env.get (i0 + 1) = 1) ∧
+    Expression.eval env x0 + Expression.eval env y0 + Expression.eval env carry_in + -env.get i0 + -(env.get (i0 + 1) * 256) = 0) ∧
+  (ZMod.val (env.get (i0 + 2)) < 256 ∧ (env.get (i0 + 3) = 0 ∨ env.get (i0 + 3) = 1) ∧
+    Expression.eval env x1 + Expression.eval env y1 + env.get (i0 + 1) + -env.get (i0 + 2) + -(env.get (i0 + 3) * 256) = 0) ∧
+  (ZMod.val (env.get (i0 + 4)) < 256 ∧ (env.get (i0 + 5) = 0 ∨ env.get (i0 + 5) = 1) ∧
+    Expression.eval env x2 + Expression.eval env y2 + env.get (i0 + 3) + -env.get (i0 + 4) + -(env.get (i0 + 5) * 256) = 0) ∧
+  (ZMod.val (env.get (i0 + 6)) < 256 ∧ (env.get (i0 + 7) = 0 ∨ env.get (i0 + 7) = 1) ∧
+    Expression.eval env x3 + Expression.eval env y3 + env.get (i0 + 5) + -env.get (i0 + 6) + -(env.get (i0 + 7) * 256) = 0) := by
 
   -- these are equivalent ways of rewriting the constraints
   -- the second one relies on prior inference of a `ExplicitCircuit` instance
@@ -38,14 +39,17 @@ example (input : Var Inputs (F p)) (env) (i0 : ℕ) :
   -- TODO on the whole, which is better?
 
   -- first version: using `circuit_norm`
-  -- dsimp only [circuit_norm, circuit32, add32_full, add8_full_carry, Boolean.circuit]
-  -- simp only [subcircuit_norm, circuit_norm]
+  -- dsimp only [circuit_norm, circuit32, add32_full, add8_full_carry, Boolean.circuit, Gadgets.ByteLookup]
+  -- simp only [subcircuit_norm, circuit_norm, Nat.reduceAdd, and_assoc]
+  -- simp only [Gadgets.ByteTable.equiv]
 
   -- second version: using `ExplicitCircuit`
   -- resolve explicit circuit operations
-  dsimp only [lawful_norm, explicit, Boolean.circuit]
-  -- simp constraints hold expression
-  simp only [append_empty, empty_append, append_assoc, append_val, Circuit.constraints_hold.append_soundness, Circuit.constraints_hold.soundness]
-  -- simp `eval` and boolean subcircuit soundness
-  simp only [subcircuit_norm, circuit_norm]
-  sorry
+  rw [ExplicitCircuit.operations_eq]
+  dsimp only [lawful_norm, explicit, Boolean.circuit, Gadgets.ByteLookup]
+  -- simp `constraints_hold` expression
+  simp only [Circuit.constraints_hold.append_soundness, Circuit.constraints_hold.soundness]
+  -- simp boolean subcircuit soundness and logical/arithmetic/vector expressions
+  simp only [subcircuit_norm, circuit_norm, Nat.reduceAdd]
+  -- finish
+  simp only [Gadgets.ByteTable.equiv]
